update proof

proof/modelT.v
@@ -8,78 +8,89 @@ Definition ThreadId := nat.
 
 (* The location is bound *)
 (* TODO: add global *)
-Definition Tlocation : Type := prod ThreadId location.
+(* Definition Tlocation : Type := prod ThreadId location. *)
 
-Definition Taccessible: Type := list Tlocation.
+(* Definition Taccessible: Type := list Tlocation. *)
 
-Definition eq_Tlocation (i1 i2: Tlocation) : bool := 
-  match i1, i2 with
-  | (tid1, l1), (tid2, l2) => if tid1 =? tid2 then eq_location l1 l2 else false
-  end.
+(* Definition eq_Tlocation (i1 i2: Tlocation) : bool :=  *)
+(*   match i1, i2 with *)
+(*   | (tid1, l1), (tid2, l2) => if tid1 =? tid2 then eq_location l1 l2 else false *)
+(*   end. *)
 
-Theorem eq_Tlocation_eq: forall i1 i2, eq_Tlocation i1 i2 = true <-> i1 = i2.
-Proof.
-  split.
-  - destruct i1 eqn:eqi1; destruct i2 eqn:eqi2; unfold eq_Tlocation; 
-    intros; try discriminate H; apply pair_equal_spec; split;
-    destruct (t =? t0) eqn: eqtt0; try apply Nat.eqb_eq; try assumption; try discriminate H. apply eq_location_eq. assumption.
-  - destruct i1 eqn:eqi1; destruct i2 eqn:eqi2; unfold eq_location; 
-    intros; inversion H. unfold eq_Tlocation. rewrite Nat.eqb_refl.
-    apply eq_location_eq. reflexivity.
-Qed.
+(* Theorem eq_Tlocation_eq: forall i1 i2, eq_Tlocation i1 i2 = true <-> i1 = i2. *)
+(* Proof. *)
+(*   split. *)
+(*   - destruct i1 eqn:eqi1; destruct i2 eqn:eqi2; unfold eq_Tlocation;  *)
+(*     intros; try discriminate H; apply pair_equal_spec; split; *)
+(*     destruct (t =? t0) eqn: eqtt0; try apply Nat.eqb_eq; try assumption; try discriminate H. apply eq_location_eq. assumption. *)
+(*   - destruct i1 eqn:eqi1; destruct i2 eqn:eqi2; unfold eq_location;  *)
+(*     intros; inversion H. unfold eq_Tlocation. rewrite Nat.eqb_refl. *)
+(*     apply eq_location_eq. reflexivity. *)
+(* Qed. *)
 
-Lemma eq_Tlocation_refl: forall (l: Tlocation), eq_Tlocation l l = true.
-Proof.
-  intros l. assert (H: l = l). reflexivity.
-  apply eq_Tlocation_eq. reflexivity.
-Qed.
+(* Lemma eq_Tlocation_refl: forall (l: Tlocation), eq_Tlocation l l = true. *)
+(* Proof. *)
+(*   intros l. assert (H: l = l). reflexivity. *)
+(*   apply eq_Tlocation_eq. reflexivity. *)
+(* Qed. *)
 
 (* ThreadId, as the owner of the cell, is stored in Tcell *)
 Inductive Tcell: Type :=
-  | TAppMem (v: tagged_value) (* note that thread isolation doesn't work on insecure memory! *)
+  | TAppMem (v: tag_value) (* note that thread isolation doesn't work on insecure memory! *)
+  | TDummyMem
   | TUnusedMem
-  | TEncMem (t: ThreadId) (z: enc_mem_tag) (v: tagged_value)
+  | TEncMem (t: ThreadId) (z: enclave_tag) (v: tag_value)
 .
 
-Definition Tmemory: Type := Tlocation -> Tcell.
+Definition Tmemory: Type := location -> Tcell.
 
 Definition empty_Tmem : Tmemory := 
   (fun _ => TUnusedMem).
 
-(* This update may not be secure! Compare tid? *)
-Definition Tupdate (s: Tlocation) (v: Tcell) (m: Tmemory) : Tmemory := 
+(* This update is secure! *)
+Definition Tupdate (t: ThreadId) (l: location) (v: Tcell) (m: Tmemory) : Tmemory := 
   match v with
+  | TDummyMem => m
   | TAppMem _ 
-  | TUnusedMem => fun s' => if (eq_Tlocation s' s) then v else m s'
-  | TEncMem t _ _ => if (fst s =? t) (*Checking if the updating is allowed! *)
-                        then fun s' => if (eq_Tlocation s' s) then v else m s'
-                        else m
+  | TUnusedMem => fun s' => if (eq_location s' l) then v else m s'
+  | TEncMem t' _ _ => if (t' =? t) (*Checking if the updating is allowed! *)
+                        then fun s' => if (eq_location s' l) then v else m s'
+                        else m  (* update failed *)
   end.
 
-Definition Taccess (me: Tmemory) (mo: mode) (s: Tlocation) : @result tagged_value := 
+Definition unsafe_update (t: ThreadId) (s: location) (v: Tcell) (m: Tmemory) : Tmemory := 
+  fun s' => if (eq_location s' s) then v else m s'.
+
+(* safe memory access *)
+Definition Taccess (t: ThreadId) (me: Tmemory) (mo: mode) (s: location) : @result tag_value := 
   let c := me s in
     match mo, c with
+    | _, TDummyMem
     | _, TUnusedMem => Err([Invalid])
     | EnclaveMode, TAppMem v => Ok v
-    (* Checking if mem of another thread is accessed *)
-    | EnclaveMode, TEncMem t _ v => if t =? (fst s) then Ok v else Err([NoPriviledge])
+    (* Checking if enclave memory of another thread is accessed *)
+    | EnclaveMode, TEncMem t' _ v => if t' =? t then Ok v else Err([NoPriviledge])
     | NormalMode, TEncMem _ _ _ => Err([NoPriviledge])
     | NormalMode, TAppMem v => Ok(v)
     end.
 
 (* We assume that only the enclave memory is thread-specific *)
-Theorem T_access_App_shared: forall (me: Tmemory) tid tid' l v,
-  me (tid, l) = TAppMem v -> me (tid', l) = TAppMem v.
+Theorem Taccess_App_shared: forall (me: Tmemory) mo (t t': ThreadId) l v,
+  me l = TAppMem v -> Taccess t' me mo l = Ok v.
 Proof.
-Admitted.
+  intros. unfold Taccess.
+  destruct mo eqn: eqmo; destruct (me l) eqn: eql; inversion H; try reflexivity.
+Qed.
 
-Theorem T_access_Unused_shared: forall (me: Tmemory) tid tid' l,
-  me (tid, l) = TUnusedMem -> me (tid', l) = TUnusedMem.
+Theorem Taccess_Unused_shared: forall (me: Tmemory) mo (t t': ThreadId) l,
+  me l = TUnusedMem -> Taccess t' me mo l = Err([Invalid]).
 Proof.
-Admitted.
+  intros. unfold Taccess.
+  destruct mo eqn: eqmo; destruct (me l) eqn: eql; inversion H; try reflexivity.
+Qed.
 
 (* secrets find on places other than the zone *)
-Fixpoint Tleaked (me: Tmemory) (vars: Taccessible) : bool := 
+Fixpoint Tleaked (me: Tmemory) (vars: accessible) : bool := 
   match vars with
   | [] => false
   | l::ls => match me l with
@@ -90,26 +101,26 @@ Fixpoint Tleaked (me: Tmemory) (vars: Taccessible) : bool :=
             end
   end.
 
-Inductive Texp: Type :=
-  | TExpLoc (l: Tlocation)
-  | TExpVal (v: value)
-  | TExpUnary (e: Texp) (op: value -> value)
-  | TExpBinary (e1 e2: Texp) (op: value -> value -> value)
-.
+(* Inductive Texp: Type := *)
+(*   | TExpLoc (l: Tlocation) *)
+(*   | TExpVal (v: value) *)
+(*   | TExpUnary (e: Texp) (op: value -> value) *)
+(*   | TExpBinary (e1 e2: Texp) (op: value -> value -> value) *)
+(* . *)
 
-Fixpoint Texp_eval (me: Tmemory) (mo: mode) (e: Texp) : @result value := 
+Fixpoint Texp_eval (t: ThreadId) (me: Tmemory) (mo: mode) (e: exp) : @result value := 
   match e with
-  | TExpLoc l => match Taccess me mo l with
+  | ExpLoc l => match Taccess t me mo l with
                 | Ok v => Ok (fst v)
                 | Err e => Err e
                 end
-  | TExpVal v => Ok(v)
-  | TExpUnary e _ => match Texp_eval me mo e with
+  | ExpVal v => Ok(v)
+  | ExpUnary e _ => match Texp_eval t me mo e with
                     | Ok _ => Ok(Any)
                     | e => e
                     end
-  | TExpBinary e1 e2 _ => let r1 := Texp_eval me mo e1 in
-                         let r2 := Texp_eval me mo e2 in
+  | ExpBinary e1 e2 _ => let r1 := Texp_eval t me mo e1 in
+                         let r2 := Texp_eval t me mo e2 in
                          match r1, r2 with
                          | Ok _, Ok _ => Ok(Any)
                          | Err er1, Err er2 => Err(er1 ++ er2)
@@ -118,114 +129,115 @@ Fixpoint Texp_eval (me: Tmemory) (mo: mode) (e: Texp) : @result value :=
                          end
   end.
 
-Definition Texp_as_bool (me: Tmemory) (mo: mode) (e: Texp) : @result bool := 
-  match Texp_eval me mo e with
+Definition Texp_as_bool (t: ThreadId) (me: Tmemory) (mo: mode) (e: exp) : @result bool := 
+  match Texp_eval t me mo e with
   | Ok v => Ok (value_as_bool v)
   | Err e => Err e
   end.
 
 
-Fixpoint Texp_prop_tag (me: Tmemory) (mo: mode) (e: Texp) : security_tag := 
+Fixpoint Texp_prop_tag (t: ThreadId) (me: Tmemory) (mo: mode) (e: exp) : security_tag := 
   match e with
-  | TExpLoc l => match Taccess me mo l with
+  | ExpLoc l => match Taccess t me mo l with
                 | Ok v => (snd v)
                 | Err e => Nonsense
                 end
-  | TExpVal v => Notsecret
-  | TExpUnary e _ => Texp_prop_tag me mo e
-  | TExpBinary e1 e2 _ =>  let t1 := Texp_prop_tag me mo e1 in
-                          let t2 := Texp_prop_tag me mo e2 in
+  | ExpVal v => Notsecret
+  | ExpUnary e _ => Texp_prop_tag t me mo e
+  | ExpBinary e1 e2 _ =>  let t1 := Texp_prop_tag t me mo e1 in
+                          let t2 := Texp_prop_tag t me mo e2 in
                           sum_two_tags t1 t2
   end.
 
-Definition Texp_tagged_val (me: Tmemory) (mo: mode) (e: Texp) : @result tagged_value := 
-  match (Texp_eval me mo e), (Texp_prop_tag me mo e) with
+Definition Texp_tagged_val (t: ThreadId) (me: Tmemory) (mo: mode) (e: exp) : @result tag_value := 
+  match (Texp_eval t me mo e), (Texp_prop_tag t me mo e) with
   | Ok v, t => Ok (v, t)
   | Err ev, _ => Err ev
   end.
 
-Inductive Tcom : Type :=
-  | TCNop
-  | TCEenter
-  | TCEexit
-  | TCAsgn (l: Tlocation) (v: Texp)
-  | TCSeq (c1 c2: Tcom)
-  | TCIf (b: Texp) (c1 c2: Tcom)
-  | TCWhile (b: Texp) (c: Tcom)
-  (* Declasification *)
-.
+(* Inductive Tcom : Type := *)
+(*   | TCNop *)
+(*   | TCEenter *)
+(*   | TCEexit *)
+(*   | TCAsgn (l: Tlocation) (v: Texp) *)
+(*   | TCSeq (c1 c2: Tcom) *)
+(*   | TCIf (b: Texp) (c1 c2: Tcom) *)
+(*   | TCWhile (b: Texp) (c: Tcom) *)
+(*   (* Declasification *) *)
+(* . *)
 
-Definition Tstate: Type := Tmemory * mode * Taccessible * errors.
+Definition Tstate: Type := Tmemory * mode * accessible * errors.
 
 (* Add tid here *)
-Inductive Tcom_eval_critical : ThreadId -> Tcom -> Tstate -> Tstate -> Prop :=
-  | TE_Nop (tid: ThreadId) (me: Tmemory) (mo: mode) (vars: Taccessible) (ers: errors) (ers: errors): 
-    Tcom_eval_critical tid TCNop (me, mo, vars, ers) (me, mo, vars, ers)
-  | TE_Eenter (tid: ThreadId) (me: Tmemory) (mo: mode) (vars: Taccessible) (ers: errors) (Her: ers = []):
-    Tcom_eval_critical tid TCEenter (me, mo, vars, ers) (me, EnclaveMode, vars, ers)
-  | TE_Eexit (tid: ThreadId) (me: Tmemory) (mo: mode) (vars: Taccessible) (ers: errors) (Her: ers = []):
-    Tcom_eval_critical tid TCEexit (me, mo, vars, ers) (me, NormalMode, vars, ers)
-  | TE_Asgn_Ok_enc (tid: ThreadId) (me: Tmemory) (mo: mode) (vars: Taccessible) (ers: errors) (Her: ers = [])
-    (l: Tlocation) (v: Texp) (r: tagged_value) 
-    (Hexp: Texp_tagged_val me mo v = (Ok r)) (Henc: mo = EnclaveMode) 
-    (Ht: (fst l) = tid) (* only assign correct tid! *):
+Inductive Tcom_eval_critical : ThreadId -> com -> Tstate -> Tstate -> Prop :=
+  | TE_Nop (tid: ThreadId) (me: Tmemory) (mo: mode) (vars: accessible) (ers: errors) (ers: errors): 
+    Tcom_eval_critical tid CNop (me, mo, vars, ers) (me, mo, vars, ers)
+  | TE_Eenter (tid: ThreadId) (me: Tmemory) (mo: mode) (vars: accessible) (ers: errors) (Her: ers = []):
+    Tcom_eval_critical tid CEenter (me, mo, vars, ers) (me, EnclaveMode, vars, ers)
+  | TE_Eexit (tid: ThreadId) (me: Tmemory) (mo: mode) (vars: accessible) (ers: errors) (Her: ers = []):
+    Tcom_eval_critical tid CEexit (me, mo, vars, ers) (me, NormalMode, vars, ers)
+  | TE_Asgn_Ok_enc (tid: ThreadId) (me: Tmemory) (mo: mode) (vars: accessible) (ers: errors) (Her: ers = [])
+    (l: location) (v: exp) (r: tag_value) 
+    (Hexp: Texp_tagged_val tid me mo v = (Ok r)) (Henc: mo = EnclaveMode) 
+    (* only assign correct tid! *):
     (* What if not in the enclave mode? *)
     (* Write restricted in the Zone! *)
-    Tcom_eval_critical tid (TCAsgn l v) (me, mo, vars, ers) ((Tupdate l (TEncMem tid ZoneMem r) me), mo, (l :: vars), ers)
-  | TE_Asgn_Err_access (tid: ThreadId) (me: Tmemory) (mo: mode) (vars: Taccessible) (ers: errors) (Her: ers = [])
-    (l: Tlocation) (v: Texp) (er: errors) (Hexp: Texp_tagged_val me mo v = (Err er)):
-    Tcom_eval_critical tid (TCAsgn l v) (me, mo, vars, ers) (me, mo, vars, (er ++ ers))
-  | TE_Seq (tid: ThreadId) (st st' st'': Tstate) (c1 c2: Tcom)
+    Tcom_eval_critical tid (CAsgn l v) (me, mo, vars, ers) ((Tupdate tid l (TEncMem tid ZoneMem r) me), mo, (l :: vars), ers)
+  | TE_Asgn_Err_access (tid: ThreadId) (me: Tmemory) (mo: mode) (vars: accessible) (ers: errors) (Her: ers = [])
+    (l: location) (v: exp) (er: errors) (Hexp: Texp_tagged_val tid me mo v = (Err er)):
+    Tcom_eval_critical tid (CAsgn l v) (me, mo, vars, ers) (me, mo, vars, (er ++ ers))
+  | TE_Seq (tid: ThreadId) (st st' st'': Tstate) (c1 c2: com)
     (Hc1: Tcom_eval_critical tid c1 st st') (Hc2: Tcom_eval_critical tid c2 st' st''):
-    Tcom_eval_critical tid (TCSeq c1 c2) st st''
-  | TE_If_then (tid: ThreadId) (me: Tmemory) (mo: mode) (vars: list Tlocation) (ers: errors) (Her: ers = [])
-    (b: Texp) (c1 c2: Tcom) (st': Tstate):
-    Texp_as_bool me mo b = Ok true -> 
+    Tcom_eval_critical tid (CSeq c1 c2) st st''
+  | TE_If_then (tid: ThreadId) (me: Tmemory) (mo: mode) (vars: list location) (ers: errors) (Her: ers = [])
+    (b: exp) (c1 c2: com) (st': Tstate):
+    Texp_as_bool tid me mo b = Ok true -> 
     Tcom_eval_critical tid c1 (me, mo, vars, ers) st' -> 
-    Tcom_eval_critical tid (TCIf b c1 c2) (me, mo, vars, ers) st'
-  | TE_If_else (tid: ThreadId) (me: Tmemory) (mo: mode) (vars: list Tlocation) (ers: errors) (Her: ers = [])
-    (b: Texp) (c1 c2: Tcom) (st': Tstate):
-    Texp_as_bool me mo b = Ok false -> 
+    Tcom_eval_critical tid (CIf b c1 c2) (me, mo, vars, ers) st'
+  | TE_If_else (tid: ThreadId) (me: Tmemory) (mo: mode) (vars: list location) (ers: errors) (Her: ers = [])
+    (b: exp) (c1 c2: com) (st': Tstate):
+    Texp_as_bool tid me mo b = Ok false -> 
     Tcom_eval_critical tid c2 (me, mo, vars, ers) st' -> 
-    Tcom_eval_critical tid (TCIf b c1 c2) (me, mo, vars, ers) st'
-  | TE_If_err (tid: ThreadId) (me: Tmemory) (mo: mode) (vars: list Tlocation) (ers: errors) (Her: ers = [])
-    (b: Texp) (c1 c2: Tcom) (st': Tstate) (er: errors):
-    Texp_as_bool me mo b = Err er -> 
-    Tcom_eval_critical tid (TCIf b c1 c2) (me, mo, vars, ers) (me, mo, vars, er ++ ers)
-  | TE_while_true (tid: ThreadId) (me: Tmemory) (mo: mode) (vars: list Tlocation) (ers: errors) (Her: ers = [])
-    (b: Texp) (c: Tcom) (st': Tstate):
-    Texp_as_bool me mo b = Ok true -> 
+    Tcom_eval_critical tid (CIf b c1 c2) (me, mo, vars, ers) st'
+  | TE_If_err (tid: ThreadId) (me: Tmemory) (mo: mode) (vars: list location) (ers: errors) (Her: ers = [])
+    (b: exp) (c1 c2: com) (st': Tstate) (er: errors):
+    Texp_as_bool tid me mo b = Err er -> 
+    Tcom_eval_critical tid (CIf b c1 c2) (me, mo, vars, ers) (me, mo, vars, er ++ ers)
+  | TE_while_true (tid: ThreadId) (me: Tmemory) (mo: mode) (vars: list location) (ers: errors) (Her: ers = [])
+    (b: exp) (c: com) (st': Tstate):
+    Texp_as_bool tid me mo b = Ok true -> 
     Tcom_eval_critical tid c (me, mo, vars, ers) st' -> 
-    Tcom_eval_critical tid (TCWhile b c) (me, mo, vars, ers) st'
-  | TE_while_false (tid: ThreadId) (me: Tmemory) (mo: mode) (vars: list Tlocation) (ers: errors) (Her: ers = [])
-    (b: Texp) (c: Tcom) (st': state):
-    Texp_as_bool me mo b = Ok false -> 
-    Tcom_eval_critical tid (TCWhile b c) (me, mo, vars, ers) (me, mo, vars, ers)
-  | TE_while_err (tid: ThreadId) (me: Tmemory) (mo: mode) (vars: list Tlocation) (ers: errors) (Her: ers = [])
-    (b: Texp) (c: Tcom) (st': state) (er: errors):
-    Texp_as_bool me mo b = Err er -> 
-    Tcom_eval_critical tid (TCWhile b c) (me, mo, vars, ers) (me, mo, vars, er ++ ers)
-  | TE_Err_ignore (tid: ThreadId) (me: Tmemory) (mo: mode) (vars: Taccessible) (ers: errors) 
-    (Herr: (length ers) >= 1) (c: Tcom):
+    Tcom_eval_critical tid (CWhile b c) (me, mo, vars, ers) st'
+  | TE_while_false (tid: ThreadId) (me: Tmemory) (mo: mode) (vars: list location) (ers: errors) (Her: ers = [])
+    (b: exp) (c: com) (st': state):
+    Texp_as_bool tid  me mo b = Ok false -> 
+    Tcom_eval_critical tid (CWhile b c) (me, mo, vars, ers) (me, mo, vars, ers)
+  | TE_while_err (tid: ThreadId) (me: Tmemory) (mo: mode) (vars: list location) (ers: errors) (Her: ers = [])
+    (b: exp) (c: com) (st': state) (er: errors):
+    Texp_as_bool tid me mo b = Err er -> 
+    Tcom_eval_critical tid (CWhile b c) (me, mo, vars, ers) (me, mo, vars, er ++ ers)
+  | TE_Err_ignore (tid: ThreadId) (me: Tmemory) (mo: mode) (vars: accessible) (ers: errors) 
+    (Herr: (length ers) >= 1) (c: com):
     Tcom_eval_critical tid c (me, mo, vars, ers) (me, mo, vars, ers)
 .
 
 (* Singlize the multi-threading state-related data structures *)
 Definition singlize_Tcell (tid: ThreadId) (c: Tcell) := 
   match c with
+  | TDummyMem => TDummyMem
   | TAppMem v => AppMem v
   | TUnusedMem => UnusedMem
   | TEncMem t z v
     => if (t =? tid) then EncMem z v else UnusedMem
   end.
 
-Fixpoint singlize_Taccessible (tid: ThreadId) (vars: Taccessible) : accessible := 
+Fixpoint singlize_accessible (tid: ThreadId) (vars: accessible) : accessible := 
   match vars with
   | [] => []
-  | h :: t => if (fst h =? tid) then (snd h) :: (singlize_Taccessible tid t) else (singlize_Taccessible tid t)
+  | h :: t => if (fst h =? tid) then (snd h) :: (singlize_accessible tid t) else (singlize_accessible tid t)
   end.
 
-Fixpoint singlize_Tmemory (tid: ThreadId) (me: Tmemory) (vars: Taccessible) : memory := 
+Fixpoint singlize_Tmemory (tid: ThreadId) (me: Tmemory) (vars: accessible) : memory := 
   match vars with
   | [] => empty_mem
   | h :: t => update (snd h) (singlize_Tcell (fst h) (me h)) (singlize_Tmemory tid me t)
@@ -263,10 +275,10 @@ Qed.
 
 Definition singlize_Tstate (tid: ThreadId) (st: Tstate) : state := 
   match st with
-  | (me, mo, vars, ers) => ((singlize_Tmemory tid me vars), mo, (singlize_Taccessible tid vars), ers)
+  | (me, mo, vars, ers) => ((singlize_Tmemory tid me vars), mo, (singlize_accessible tid vars), ers)
   end.
 
-Fixpoint singlize_Texp (te: Texp) : exp :=
+Fixpoint singlize_Texp (te: exp) : exp :=
   match te with
   | TExpLoc l => ExpLoc (snd l)
   | TExpVal v => ExpVal v
@@ -325,7 +337,7 @@ Proof.
   (* Eexit *)
   - simpl. apply E_Eexit. assumption.
   (* Asgn *)
-  - simpl. destruct l. simpl in *. subst. rewrite <- beq_nat_refl with tid in *. rewrite eq_Tlocation_refl.
+  - simpl. destruct l. simpl in *. subst. rewrite <- beq_nat_refl with tid in *. rewrite eq_location_refl.
     simpl. rewrite <- beq_nat_refl with tid. admit.
   - apply E_Asgn_Err_access. assumption. 
   apply Texp_eval_singlize_err_prop in Hexp. admit.
